lakefile.lean
@@ -1,10 +1,12 @@
 import Lake
 open Lake DSL
 
-package urf_core
+package urf_spine where
+  leanOptions := #[⟨`pp.unicode.fun, true⟩]
 
-require mathlib from git
-  "https://github.com/leanprover-community/mathlib4.git"
+require mathlib from
+  git "https://github.com/leanprover-community/mathlib4"
+  @ "a3a10db0e9d66acbebf76c5e6a135066525ac900"
 
 @[default_target]
 lean_lib URFSpine where
